\documentclass{article}
\usepackage{graphicx} % Required for inserting images
\usepackage{amsmath}
\usepackage{geometry}
\geometry{legalpaper, landscape, margin=1in}
\title{cases-verification}
\author{haiml76 }
\date{December 2025}

\begin{document}

\maketitle
\section{}

\section{}
$v_1\geq{v_3}\geq{0}\Rightarrow{v_{11}}\geq{-v_2-v_3}$

$v_1\geq{v_4}>v_2\geq{0}\Rightarrow\alpha:=\min\{v_2,v_2+v_{11}+v_1\}=\begin{cases}
v_2,&v_{11}\geq{-v_1}\\
v_2-1,v_2-2,\dots,&v_{11}<{-v_1}\\
    \end{cases}$

     $v_1\geq{v_4}>v_2\geq{0}\Rightarrow{f(p,t)=p^{7v_1+10v_2+11v_3+7v_4+v_4}t^{4v_1+6v_2+6v_3+4v_4}=p^{7v_1+10v_2+11v_3+8v_4}t^{4v_1+6v_2+6v_3+4v_4}}$
\subsection{}
\subsection{$-v_2-v_3<{-v_1}<-v_2\Rightarrow{v_1<{v_2+v_3}}$}
\[\begin{matrix}
v_{11}\geq{-v_2}&p^{\min\{0,\geq{v_2}-v_2\}}=p^0=1&\alpha=\min\{v_2,\geq{v_1}\}=v_2&\mu(a_{11})=p^{v_2}\\
v_{11}={-(v_2+1)}&p^{\min\{0,v_2-(v_2+1)\}}=p^{-1}&\alpha=\min\{v_2,v_1-1\}=v_2&\mu(a_{11})=p^{v_2+1}-p^{v_2}=p^{v_2+1}(1-p^{-1})\\
v_{11}={-(v_2+1)}&p^{\min\{0,v_2-(v_2+2)\}}=p^{-2}&\alpha=\min\{v_2,v_1-2\}=v_2&\mu(a_{11})=p^{v_2+2}-p^{v_2+1}=p^{v_2+2}(1-p^{-1})\\
\vdots&\vdots&\vdots&\vdots\\
v_{11}=-v_1&p^{\min\{0,v_2-v_1\}}=p^{v_2-v_1}&\alpha=\min\{v_2,v_1-v_1+v_2\}=v_2&\mu(a_{11})=p^{v_1}-p^{v_1-1}=p^{v_1}(1-p^{-1})\\
v_{11}=-(v_1+1)&p^{\min\{0,v_2-(v_1+1)\}}=p^{v_2-(v_1+1)}&\alpha=\min\{v_2,v_1-(v_1+1)+v_2\}=v_2-1&\mu(a_{11})=p^{v_1+1}-p^{v_1}=p^{v_1+1}(1-p^{-1})\\
v_{11}=-(v_1+2)&p^{\min\{0,v_2-(v_1+2)}=p^{v_2-(v_1+2)}&\alpha=\min\{v_2,v_1-(v_1+2)+v_2\}=v_2-2&\mu(a_{11})=p^{v_1+2}-p^{v_1+1}=p^{v_1+2}(1-p^{-1})\\
\vdots&\vdots&\vdots&\vdots\\
v_{11}=-(v_2+v_3)&p^{\min\{0,v_2-(v_2+v_3)\}}=p^{-v_3}&\alpha=\min\{v_2,v_1-(v_2+v_3)+v_2\}=v_1-v_3&\mu(a_{11})=p^{v_2+v_3}-p^{v_2+v_3-1}=p^{v_2+v_3}(1-p^{-1})\\
\end{matrix}\]

\begin{enumerate}
    \item $p^{v_2}(1+v_2A)$.
    \item $\sum_{-v_{11}=v_2+1}^{v_1}p^{v_2}A(1+v_2A)=(v_1-v_2)(A+v_2A^2)=(v_1-v_2)p^{v_2}(A+v_2A^2)=p^{v_2}(v_1A-v_2A+v_1v_2A^2-v_2^2A^2)$.
    \item $\sum_{-v_{11}=v_1+1}^{v_2+v_3}p^{v_2}A(1+(v_1+v_2+v_{11})A)=\sum_{i=1}^{v_2+v_3-v_1}p^{v_2}A(1+(v_2-i)A)=\sum_{i=1}^{v_2+v_3-v_1}p^{v_2}A+\sum_{i=1}^{v_2+v_3-v_1}p^{v_2}A((v_2-i)A)=$
    
    $=\sum_{i=1}^{v_2+v_3-v_1}p^{v_2}A+\sum_{i=1}^{v_2+v_3-v_1}p^{v_2}A(v_2A-iA)=\sum_{i=1}^{v_2+v_3-v_1}p^{v_2}A+\sum_{i=1}^{v_2+v_3-v_1}p^{v_2}A^2v_2-\sum_{i=1}^{v_2+v_3-v_1}p^{v_2}A^2i=$
    
    $=(v_2+v_3-v_1)p^{v_2}A+(v_2+v_3-v_1)p^{v_2}A^2v_2-\frac{(v_2+v_3-v_1)(v_2+v_3-v_1+1)}{2}p^{v_2}A^2=$
    
    $=p^{v_2}(v_2A+v_3A-v_1A+v_2^2A^2+v_3v_2A^2-v_1v_2A^2-A^2(\frac{v_2^2}{2}+\frac{v_2v_3}{2}-\frac{v_2v_1}{2}+\frac{v_3v_2}{2}+\frac{v_3^2}{2}-\frac{v_3v_1}{2}-\frac{v_1v_2}{2}-\frac{v_1v_3}{2}+\frac{v_1^2}{2}+$
    
    $+\frac{v_2}{2}+\frac{v_3}{2}-\frac{v_1}{2})=p^{v_2}(v_2A+v_3A-v_1A+v_2^2A^2+v_3v_2A^2-v_1v_2A^2-A^2(\frac{v_2^2}{2}+v_2v_3-v_2v_1+\frac{v_3^2}{2}-v_3v_1+\frac{v_1^2}{2}+\frac{v_2}{2}+\frac{v_3}{2}-\frac{v_1}{2})=$
    
    $=p^{v_2}(v_2A+v_3A-v_1A+v_2^2A^2+v_3v_2A^2-v_1v_2A^2-\frac{v_2^2}{2}A^2-v_2v_3A^2+v_2v_1A^2-\frac{v_3^2}{2}A^2+v_3v_1A^2-\frac{v_1^2}{2}A^2-\frac{v_2}{2}A^2-\frac{v_3}{2}A^2+\frac{v_1}{2}A^2)=$
    
    $=p^{v_2}(v_2A+v_3A-v_1A+\frac{v_2^2}{2}A^2-\frac{v_3^2}{2}A^2+v_3v_1A^2-\frac{v_1^2}{2}A^2-\frac{v_2}{2}A^2-\frac{v_3}{2}A^2+\frac{v_1}{2}A^2).
    $
\end{enumerate}
Thus, our polynomial is

$p^{v_2}(1+v_2A+v_1A-v_2A+v_1v_2A^2-v_2^2A^2+v_2A+v_3A-v_1A+\frac{v_2^2}{2}A^2-\frac{v_3^2}{2}A^2+v_3v_1A^2-\frac{v_1^2}{2}A^2-\frac{v_2}{2}A^2-\frac{v_3}{2}A^2+\frac{v_1}{2}A^2)=$

$=p^{v_2}(1+v_1v_2A^2-\frac{v_2^2}{2}A^2+v_2A+v_3A-\frac{v_3^2}{2}A^2+v_3v_1A^2-\frac{v_1^2}{2}A^2-\frac{v_2}{2}A^2-\frac{v_3}{2}A^2+\frac{v_1}{2}A^2)$.
\section{}
$v_3>v_1\geq{0}\implies{v_{11}}\geq{-v_2-v_1}$

$v_4>v_1\geq{0}$

$v_4>v_2\geq{0}$

$\Rightarrow\alpha:=\min\{v_2,v_2+v_{11}+v_4\}=\begin{cases}
       v_2, & v_{11}\geq{-v_4}\\
       v_2-1,v_2-2,\dots, & v_{11}<{-v_4}\\
     \end{cases}$

     $\Rightarrow{f(p,t)=p^{7v_1+10v_2+11v_3+7v_4+v_1}t^{4v_1+6v_2+6v_3+4v_4}=p^{8v_1+10v_2+11v_3+7v_4}t^{4v_1+6v_2+6v_3+4v_4}}$
\subsection{$-v_2-v_1>-v_4\implies{v_4>v_2+v_1}$}
\[\begin{matrix}
v_{11}\geq{-v_2}&p^{\min\{0,\geq({v_2}-v_2)\}}=p^0=1&\alpha=\min\{v_2,\geq{v_4}\}=v_2&\mu(a_{11})=p^{v_2}\\
v_{11}={-(v_2+1)}&p^{\min\{0,v_2-(v_2+1)\}}=p^{-1}&\alpha=\min\{v_2,v_4-1\}=v_2&\mu(a_{11})=p^{v_2+1}-p^{v_2}=p^{v_2+1}(1-p^{-1})\\
v_{11}={-(v_2+2)}&p^{\min\{0,v_2-(v_2+2)\}}=p^{-2}&\alpha=\min\{v_2,v_4-2\}=v_2&\mu(a_{11})=p^{v_2+1}-p^{v_2}=p^{v_2+2}(1-p^{-1})\\
\vdots&\vdots&\vdots&\vdots\\
v_{11}={-(v_2+v_1)}&p^{\min\{0,v_2-(v_2+v_1)\}}=p^{-v_1}&\alpha=\min\{v_2,v_4-v_1\}=v_2&\mu(a_{11})=p^{v_2+v_1}-p^{v_2}=p^{v_2+v_1}(1-p^{-1})\\
\end{matrix}\]

\begin{enumerate}
    \item $p^{v_2}(1+v_2A)$
    \item $p^{v_2}A(1+v_2A)v_1=p^{v_2}(A+v_2A^2)v_1=p^{v_2}(v_1A+v_1v_2A^2)$.
\end{enumerate}

Thus, our polynomial is:

$p^{v_2}(1+v_2A+v_1A+v_1v_2A^2)$.
\subsection{$-v_4\geq{-v_2-v_1}\implies{v_2+v_1\geq{v_4}}$}
\[\begin{matrix}
v_{11}\geq{-v_2}&p^{\min\{0,\geq({v_2}-v_2)\}}=p^0=1&\alpha=\min\{v_2,\geq{v_4}\}=v_2&\mu(a_{11})=p^{v_2}\\
v_{11}={-(v_2+1)}&p^{\min\{0,v_2-(v_2+1)\}}=p^{-1}&\alpha=\min\{v_2,v_4-1\}=v_2&\mu(a_{11})=p^{v_2+1}-p^{v_2}=p^{v_2+1}(1-p^{-1})\\
v_{11}={-(v_2+2)}&p^{\min\{0,v_2-(v_2+2)\}}=p^{-2}&\alpha=\min\{v_2,v_4-2\}=v_2&\mu(a_{11})=p^{v_2+2}-p^{v_2}=p^{v_2+2}(1-p^{-1})\\
\vdots&\vdots&\vdots&\vdots\\
v_{11}={-v_4}&p^{\min\{0,v_2-v_4\}}=p^{v_2-v_4}&\alpha=\min\{v_2,v_2-v_4+v_4\}=v_2&\mu(a_{11})=p^{v_4}-p^{v_4-1}=p^{v_4}(1-p^{-1})\\
v_{11}={-(v_4+1)}&p^{\min\{0,v_2-(v_4+1)\}}=p^{v_2-(v_4+1)}&\alpha=\min\{v_2,v_2-(v_4+1)+v_4\}=v_2-1&\mu(a_{11})=p^{v_4+1}-p^{v_4}=p^{v_4+1}(1-p^{-1})\\
v_{11}={-(v_4+2)}&p^{\min\{0,v_2-(v_4+2)\}}=p^{v_2-(v_4+2)}&\alpha=\min\{v_2,v_2-(v_4+2)+v_4\}=v_2-2&\mu(a_{11})=p^{v_4+2}-p^{v_4+1}=p^{v_4+2}(1-p^{-1})\\
\vdots&\vdots&\vdots&\vdots\\
v_{11}={-(v_2+v_1)}&p^{\min\{0,v_2-(v_2+v_1)\}}=p^{-v_1}&\alpha=\min\{v_2,v_2-(v_2+v_1)+v_4\}=v_4-v_1&\mu(a_{11})=p^{v_2+v_1}-p^{v_2+v_1-1}=p^{v_2+v_1}(1-p^{-1})\\
\end{matrix}\]
\begin{enumerate}
    \item $p^{v_2}(1+v_2A)$.
    \item $\sum_{-v_{11}=v_2+1}^{v_4}p^{v_2}A(1+v_2A)=(v_4-v_2)(A+v_2A^2)=(v_4-v_2)p^{v_2}(A+v_2A^2)=p^{v_2}(v_4A-v_2A+v_4v_2A^2-v_2^2A^2)$.
    \item $\sum_{-v_{11}=v_4+1}^{v_2+v_1}p^{v_2}A(1+(v_4+v_2+v_{11})A)=\sum_{i=1}^{v_2+v_1-v_4}p^{v_2}A(1+(v_2-i)A)=\sum_{i=1}^{v_2+v_1-v_4}p^{v_2}A+\sum_{i=1}^{v_2+v_1-v_4}p^{v_2}A((v_2-i)A)=$

    $=\sum_{i=1}^{v_2+v_1-v_4}p^{v_2}A+\sum_{i=1}^{v_2+v_1-v_4}p^{v_2}A(v_2A-iA)=\sum_{i=1}^{v_2+v_1-v_4}p^{v_2}A+\sum_{i=1}^{v_2+v_1-v_4}p^{v_2}A^2v_2-\sum_{i=1}^{v_2+v_1-v_4}p^{v_2}A^2i=$

    $=(v_2+v_1-v_4)p^{v_2}A+(v_2+v_1-v_4)p^{v_2}A^2v_2-\frac{(v_2+v_1-v_4)(v_2+v_1-v_4+1)}{2}p^{v_2}A^2=$
    
    $=p^{v_2}(v_2A+v_1A-v_4A+v_2^2A^2+v_1v_2A^2-v_4v_2A^2-A^2(\frac{v_2^2}{2}+\frac{v_2v_1}{2}-\frac{v_2v_4}{2}+\frac{v_1v_2}{2}+\frac{v_1^2}{2}-\frac{v_1v_4}{2}-\frac{v_4v_2}{2}-\frac{v_4v_1}{2}+\frac{v_4^2}{2}+$

    $+\frac{v_2}{2}+\frac{v_1}{2}-\frac{v_4}{2})=p^{v_2}(v_2A+v_1A-v_4A+v_2^2A^2+v_1v_2A^2-v_4v_2A^2-A^2(\frac{v_2^2}{2}+v_2v_1-v_2v_4+\frac{v_4^2}{2}-v_4v_1+\frac{v_1^2}{2}+\frac{v_2}{2}+\frac{v_1}{2}-\frac{v_4}{2})=$

    $=p^{v_2}(v_2A+v_1A-v_4A+v_2^2A^2+v_1v_2A^2-v_4v_2A^2-\frac{v_2^2}{2}A^2-v_2v_1A^2+v_2v_4A^2-\frac{v_4^2}{2}A^2+v_4v_1A^2-\frac{v_1^2}{2}A^2-\frac{v_2}{2}A^2-\frac{v_1}{2}A^2+\frac{v_4}{2}A^2)=$
    
    $=p^{v_2}(v_2A+v_1A-v_4A+\frac{v_2^2}{2}A^2-\frac{v_4^2}{2}A^2+v_4v_1A^2-\frac{v_1^2}{2}A^2-\frac{v_2}{2}A^2-\frac{v_1}{2}A^2+\frac{v_4}{2}A^2).$
    \end{enumerate}
    Thus, our polynomial is

$p^{v_2}(1+v_2A+v_4A-v_2A+v_4v_2A^2-v_2^2A^2+v_2A+v_1A-v_4A-\frac{v_2^2}{2}A^2-\frac{v_4^2}{2}A^2+v_4v_1A^2-\frac{v_1^2}{2}A^2-\frac{v_2}{2}A^2-\frac{v_1}{2}A^2+\frac{v_4}{2}A^2)=$

$=p^{v_2}(1+v_4v_2A^2-\frac{v_2^2}{2}A^2+v_2A+v_1A-\frac{v_4^2}{2}A^2+v_4v_1A^2-\frac{v_1^2}{2}A^2-\frac{v_2}{2}A^2-\frac{v_1}{2}A^2+\frac{v_4}{2}A^2)$.
\section{}
$v_4>v_1\geq{v_3}\geq{0}$

$v_4>v_2\geq{0}$

$\Rightarrow{v_{11}}\geq{-v_2-v_3}$

$\Rightarrow\alpha:=\min\{v_2,v_2+v_{11}+v_4\}=\begin{cases}
       v_2, & v_{11}\geq{-v_4}\\
       v_2-1,v_2-2,\dots, & v_{11}<{-v_4}\\
     \end{cases}$

     $\Rightarrow{f(p,t)=p^{7v_1+10v_2+11v_3+7v_4+v_1}t^{4v_1+6v_2+6v_3+4v_4}=p^{8v_1+10v_2+11v_3+7v_4}t^{4v_1+6v_2+6v_3+4v_4}}$
\subsection{$-v_4<-v_2-v_3\Rightarrow{v_4>v_2+v_3}$}
\[\begin{matrix}
v_{11}\geq{-v_2}&p^{\min\{0,\geq({v_2}-v_2)\}}=p^0=1&\alpha=\min\{v_2,\geq{v_4}\}=v_2&\mu(a_{11})=p^{v_2}\\
v_{11}={-(v_2+1)}&p^{\min\{0,v_2-(v_2+1)\}}=p^{-1}&\alpha=\min\{v_2,v_4-1\}=v_2&\mu(a_{11})=p^{v_2+1}-p^{v_2}=p^{v_2+1}(1-p^{-1})\\
v_{11}={-(v_2+2)}&p^{\min\{0,v_2-(v_2+2)\}}=p^{-2}&\alpha=\min\{v_2,v_4-2\}=v_2&\mu(a_{11})=p^{v_2+1}-p^{v_2}=p^{v_2+2}(1-p^{-1})\\
\vdots&\vdots&\vdots&\vdots\\
v_{11}={-(v_2+v_3)}&p^{\min\{0,v_2-(v_2+v_3)\}}=p^{-v_1}&\alpha=\min\{v_2,v_4-v_3\}=v_2&\mu(a_{11})=p^{v_2+v_3}-p^{v_2}=p^{v_2+v_3}(1-p^{-1})\\
\end{matrix}\]

\begin{enumerate}
    \item $p^{v_2}(1+v_2A)$
    \item $p^{v_2}A(1+v_2A)v_3=p^{v_2}(A+v_2A^2)v_3=p^{v_2}(v_3A+v_3v_2A^2)$.
\end{enumerate}

Thus, our polynomial is:

$p^{v_2}(1+v_2A+v_3A+v_3v_2A^2)$.
\subsection{$-v_4\geq-v_2-v_3\Rightarrow{v_2+v_3\geq{v_4}}$}
\[\begin{matrix}
v_{11}\geq{-v_2}&p^{\min\{0,\geq({v_2}-v_2)\}}=p^0=1&\alpha=\min\{v_2,\geq{v_4}\}=v_2&\mu(a_{11})=p^{v_2}\\
v_{11}={-(v_2+1)}&p^{\min\{0,v_2-(v_2+1)\}}=p^{-1}&\alpha=\min\{v_2,v_4-1\}=v_2&\mu(a_{11})=p^{v_2+1}-p^{v_2}=p^{v_2+1}(1-p^{-1})\\
v_{11}={-(v_2+2)}&p^{\min\{0,v_2-(v_2+2)\}}=p^{-2}&\alpha=\min\{v_2,v_4-2\}=v_2&\mu(a_{11})=p^{v_2+2}-p^{v_2}=p^{v_2+2}(1-p^{-1})\\
\vdots&\vdots&\vdots&\vdots\\
v_{11}={-v_4}&p^{\min\{0,v_2-v_4\}}=p^{v_2-v_4}&\alpha=\min\{v_2,v_2-v_4+v_4\}=v_2&\mu(a_{11})=p^{v_4}-p^{v_4-1}=p^{v_4}(1-p^{-1})\\
v_{11}={-(v_4+1)}&p^{\min\{0,v_2-(v_4+1)\}}=p^{v_2-(v_4+1)}&\alpha=\min\{v_2,v_2-(v_4+1)+v_4\}=v_2-1&\mu(a_{11})=p^{v_4+1}-p^{v_4}=p^{v_4+1}(1-p^{-1})\\
v_{11}={-(v_4+2)}&p^{\min\{0,v_2-(v_4+2)\}}=p^{v_2-(v_4+2)}&\alpha=\min\{v_2,v_2-(v_4+2)+v_4\}=v_2-2&\mu(a_{11})=p^{v_4+2}-p^{v_4+1}=p^{v_4+2}(1-p^{-1})\\
\vdots&\vdots&\vdots&\vdots\\
v_{11}={-(v_2+v_3)}&p^{\min\{0,v_2-(v_2+v_3)\}}=p^{-v_3}&\alpha=\min\{v_2,v_2-(v_2+v_3)+v_4\}=v_4-v_3&\mu(a_{11})=p^{v_2+v_3}-p^{v_2+v_3-1}=p^{v_2+v_3}(1-p^{-1})\\
\end{matrix}\]
\begin{enumerate}
    \item $p^{v_2}(1+v_2A)$.
    \item $\sum_{-v_{11}=v_2+1}^{v_4}p^{v_2}A(1+v_2A)=(v_4-v_2)p^{v_2}(A+v_2A^2)=p^{v_2}(v_4A-v_2A+v_4v_2A^2-v_2^2A^2)$.
    \item $\sum_{-v_{11}=v_4+1}^{v_2+v_3}p^{v_2}A(1+(v_4+v_2+v_{11})A)=\sum_{i=1}^{v_2+v_3-v_4}p^{v_2}A(1+(v_2-i)A)=\sum_{i=1}^{v_2+v_3-v_4}p^{v_2}A+\sum_{i=1}^{v_2+v_3-v_4}p^{v_2}A((v_2-i)A)=$

    $=\sum_{i=1}^{v_2+v_3-v_4}p^{v_2}A+\sum_{i=1}^{v_2+v_3-v_4}p^{v_2}A(v_2A-iA)=\sum_{i=1}^{v_2+v_3-v_4}p^{v_2}A+\sum_{i=1}^{v_2+v_3-v_4}p^{v_2}A^2v_2-\sum_{i=1}^{v_2+v_3-v_4}p^{v_2}A^2i=$

    $=(v_2+v_3-v_4)p^{v_2}A+(v_2+v_3-v_4)p^{v_2}A^2v_2-\frac{(v_2+v_3-v_4)(v_2+v_3-v_4+1)}{2}p^{v_2}A^2=$
    
    $=p^{v_2}(v_2A+v_3A-v_4A+v_2^2A^2+v_3v_2A^2-v_4v_2A^2-A^2(\frac{v_2^2}{2}+\frac{v_2v_3}{2}-\frac{v_2v_4}{2}+\frac{v_3v_2}{2}+\frac{v_3^2}{2}-\frac{v_3v_4}{2}-\frac{v_4v_2}{2}-\frac{v_4v_3}{2}+\frac{v_4^2}{2}+$

    $+\frac{v_2}{2}+\frac{v_3}{2}-\frac{v_4}{2})=p^{v_2}(v_2A+v_3A-v_4A+v_2^2A^2+v_3v_2A^2-v_4v_2A^2-A^2(\frac{v_2^2}{2}+v_2v_3-v_2v_4+\frac{v_4^2}{2}-v_4v_3+\frac{v_3^2}{2}+\frac{v_2}{2}+\frac{v_3}{2}-\frac{v_4}{2})=$

    $=p^{v_2}(v_2A+v_3A-v_4A+v_2^2A^2+v_3v_2A^2-v_4v_2A^2-\frac{v_2^2}{2}A^2-v_2v_3A^2+v_2v_4A^2-\frac{v_4^2}{2}A^2+v_4v_3A^2-\frac{v_3^2}{2}A^2-\frac{v_2}{2}A^2-\frac{v_3}{2}A^2+\frac{v_4}{2}A^2)=$
    
    $=p^{v_2}(v_2A+v_3A-v_4A+\frac{v_2^2}{2}A^2-\frac{v_4^2}{2}A^2+v_4v_3A^2-\frac{v_3^2}{2}A^2-\frac{v_2}{2}A^2-\frac{v_3}{2}A^2+\frac{v_4}{2}A^2).$
    \end{enumerate}
    Thus, our polynomial is

$p^{v_2}(1+v_2A+v_4A-v_2A+v_4v_2A^2-v_2^2A^2+v_2A+v_3A-v_4A+\frac{v_2^2}{2}A^2-\frac{v_4^2}{2}A^2+v_4v_3A^2-\frac{v_3^2}{2}A^2-\frac{v_2}{2}A^2-\frac{v_3}{2}A^2+\frac{v_4}{2}A^2)=$

$=p^{v_2}(1+v_4v_2A^2-\frac{v_2^2}{2}A^2+v_2A+v_3A-\frac{v_4^2}{2}A^2+v_4v_3A^2-\frac{v_3^2}{2}A^2-\frac{v_2}{2}A^2-\frac{v_3}{2}A^2+\frac{v_4}{2}A^2)$.
\section{}
\section{}
\section{}
\section{}$v_2\geq{v_4}\geq{0}$

$v_1\geq{v_4}\geq{0}$

$v_1\geq{v_3}\geq{0}$

$\Rightarrow{v_{11}}\geq{-v_2-v_3}$

$\Rightarrow\alpha:=\min\{v_4,v_2+v_{11}+v_1\}=\begin{cases}
       v_4, & v_{11}\geq{v_4-v_1-v_2}\\
       v_4-1,v_4-2,\dots, & v_{11}<{v_4-v_1-v_2}\\
     \end{cases}$

     $\Rightarrow{f(p,t)=p^{7v_1+10v_2+11v_3+7v_4+v_4}t^{4v_1+6v_2+6v_3+4v_4}=p^{7v_1+10v_2+11v_3+8v_4}t^{4v_1+6v_2+6v_3+4v_4}}$
\subsection{$v_1-v_3\geq{v_4}\iff{v_1}\geq{v_3+v_4}$}
\[\begin{matrix}
v_{11}\geq{-v_2}&p^{\min\{0,\geq({v_2}-v_2)\}}=p^0=1&\alpha=\min\{v_4,\geq{v_1}\}=v_4&\mu(a_{11})=p^{v_2}\\
v_{11}={-(v_2+1)}&p^{\min\{0,v_2-(v_2+1)\}}=p^{-1}&\alpha=\min\{v_4,v_1-1\}=v_4&\mu(a_{11})=p^{v_2+1}-p^{v_2}=p^{v_2+1}(1-p^{-1})\\
v_{11}={-(v_2+2)}&p^{\min\{0,v_2-(v_2+2)\}}=p^{-2}&\alpha=\min\{v_4,v_1-2\}=v_4&\mu(a_{11})=p^{v_2+1}-p^{v_2}=p^{v_2+2}(1-p^{-1})\\
\vdots&\vdots&\vdots&\vdots\\
v_{11}={-(v_2+v_3)}&p^{\min\{0,v_2-(v_2+v_3)\}}=p^{-v_3}&\alpha=\min\{v_4,v_2-(v_2+v_3)+v_{1}\}=v_4&\mu(a_{11})=p^{v_2+v_3}-p^{v_2}=p^{v_2+v_3}(1-p^{-1})\\
\end{matrix}\]

\begin{enumerate}
    \item $p^{v_2}(1+v_4A)$
    \item $p^{v_2}A(1+v_4A)v_3=p^{v_2}(A+v_4A^2)v_3=p^{v_2}(v_3A+v_3v_4A^2)$.
\end{enumerate}

Thus, our polynomial is:

$p^{v_2}(1+v_4A+v_3A+v_3v_4A^2)$.
\subsection{$v_1<v_3+v_4\iff{-v_3-v_4<-v_1}$}
\[\begin{matrix}
v_{11}\geq{-v_2}&p^{\min\{0,\geq({v_2}-v_2)\}}=p^0=1&\alpha=\min\{v_4,\geq{v_1}\}=v_4&\mu(a_{11})=p^{v_2}\\
v_{11}={-(v_2+1)}&p^{\min\{0,v_2-(v_2+1)\}}=p^{-1}&\alpha=\min\{v_4,v_1-1\}=v_4&\mu(a_{11})=p^{v_2+1}-p^{v_2}=p^{v_2+1}(1-p^{-1})\\
v_{11}={-(v_2+2)}&p^{\min\{0,v_2-(v_2+2)\}}=p^{-2}&\alpha=\min\{v_4,v_1-2\}=v_4&\mu(a_{11})=p^{v_2+2}-p^{v_2}=p^{v_2+2}(1-p^{-1})\\
\vdots&\vdots&\vdots&\vdots\\
v_{11}={-(v_2+v_1-v_4)}&p^{\min\{0,v_2-(v_2+v_1-v_4)\}}=p^{v_4-v_1}&\alpha=\min\{v_4,v_2-(v_2+v_1-v_4)+v_1\}=v_4&\mu(a_{11})=p^{v_2+v_1-v_4}-p^{v_2+v_1-v_4-1}=p^{v_2+v_1-v_4}(1-p^{-1})\\
v_{11}={-(v_2+v_1-v_4+1)}&p^{\min\{0,v_2-(v_2+v_1-v_4+1)\}}=p^{v_4-v_1-1}&\alpha=\min\{v_4,v_2-(v_2+v_1-v_4+1)+v_1\}=v_4-1&\mu(a_{11})=p^{v_4+1}-p^{v_4}=p^{v_4+1}(1-p^{-1})\\
v_{11}={-(v_2+v_1-v_4+2)}&p^{\min\{0,v_2-(v_2+v_1-v_4+2)\}}=p^{v_4-v_1-2}&\alpha=\min\{v_2,v_2-(v_2+v_1-v_4+2)+v_1\}=v_4-2&\mu(a_{11})=p^{v_4+2}-p^{v_4+1}=p^{v_4+2}(1-p^{-1})\\
\vdots&\vdots&\vdots&\vdots\\
v_{11}={-(v_2+v_3)}&p^{\min\{0,v_2-(v_2+v_3)\}}=p^{-v_3}&\alpha=\min\{v_2,v_2-(v_2+v_3)+v_4\}=v_4-v_3&\mu(a_{11})=p^{v_2+v_3}-p^{v_2+v_3-1}=p^{v_2+v_3}(1-p^{-1})\\
\end{matrix}\]
\begin{enumerate}
    \item $p^{v_2}(1+v_2A)$.
    \item $\sum_{-v_{11}=v_2+1}^{v_4}p^{v_2}A(1+v_2A)=(v_4-v_2)(A+v_2A^2)=(v_4-v_2)p^{v_2}(A+v_2A^2)=p^{v_2}(v_4A-v_2A+v_4v_2A^2-v_2^2A^2)$.
    \item $\sum_{-v_{11}=v_4+1}^{v_2+v_3}p^{v_2}A(1+(v_4+v_2+v_{11})A)=\sum_{i=1}^{v_2+v_3-v_4}p^{v_2}A(1+(v_2-i)A)=\sum_{i=1}^{v_2+v_3-v_4}p^{v_2}A+\sum_{i=1}^{v_2+v_3-v_4}p^{v_2}A((v_2-i)A)=$

    $=\sum_{i=1}^{v_2+v_3-v_4}p^{v_2}A+\sum_{i=1}^{v_2+v_3-v_4}p^{v_2}A(v_2A-iA)=\sum_{i=1}^{v_2+v_3-v_4}p^{v_2}A+\sum_{i=1}^{v_2+v_3-v_4}p^{v_2}A^2v_2-\sum_{i=1}^{v_2+v_3-v_4}p^{v_2}A^2i=$

    $=(v_2+v_3-v_4)p^{v_2}A+(v_2+v_3-v_4)p^{v_2}A^2v_2-\frac{(v_2+v_3-v_4)(v_2+v_3-v_4+1)}{2}p^{v_2}A^2=$
    
    $=p^{v_2}(v_2A+v_3A-v_4A+v_2^2A^2+v_3v_2A^2-v_4v_2A^2-A^2(\frac{v_2^2}{2}+\frac{v_2v_3}{2}-\frac{v_2v_4}{2}+\frac{v_3v_2}{2}+\frac{v_3^2}{2}-\frac{v_3v_4}{2}-\frac{v_4v_2}{2}-\frac{v_4v_3}{2}+\frac{v_4^2}{2}+$

    $+\frac{v_2}{2}+\frac{v_3}{2}-\frac{v_4}{2})=p^{v_2}(v_2A+v_3A-v_4A+v_2^2A^2+v_3v_2A^2-v_4v_2A^2-A^2(\frac{v_2^2}{2}+v_2v_3-v_2v_4+\frac{v_4^2}{2}-v_4v_3+\frac{v_3^2}{2}+\frac{v_2}{2}+\frac{v_3}{2}-\frac{v_4}{2})=$

    $=p^{v_2}(v_2A+v_3A-v_4A+v_2^2A^2+v_3v_2A^2-v_4v_2A^2-\frac{v_2^2}{2}A^2-v_2v_3A^2+v_2v_4A^2-\frac{v_4^2}{2}A^2+v_4v_3A^2-\frac{v_3^2}{2}A^2-\frac{v_2}{2}A^2-\frac{v_3}{2}A^2+\frac{v_4}{2}A^2)=$
    
    $=p^{v_2}(v_2A+v_3A-v_4A+\frac{v_2^2}{2}A^2-\frac{v_4^2}{2}A^2+v_4v_3A^2-\frac{v_3^2}{2}A^2-\frac{v_2}{2}A^2-\frac{v_3}{2}A^2+\frac{v_4}{2}A^2).$
    \end{enumerate}
    Thus, our polynomial is

$p^{v_2}(1+v_2A+v_4A-v_2A+v_4v_2A^2-v_2^2A^2+v_2A+v_3A-v_4A+\frac{v_2^2}{2}A^2-\frac{v_4^2}{2}A^2+v_4v_3A^2-\frac{v_3^2}{2}A^2-\frac{v_2}{2}A^2-\frac{v_3}{2}A^2+\frac{v_4}{2}A^2)=$

$=p^{v_2}(1+v_4v_2A^2-\frac{v_2^2}{2}A^2+v_2A+v_3A-\frac{v_4^2}{2}A^2+v_4v_3A^2-\frac{v_3^2}{2}A^2-\frac{v_2}{2}A^2-\frac{v_3}{2}A^2+\frac{v_4}{2}A^2)$.
\end{document}
