
                \documentclass{article}
                \usepackage{graphicx} % Required for inserting images
                \begin{document}
                \[\sum_{a\geq{0}}(p^{37}t^{20})^{a}=\frac{(1)}{(1-p^{37}t^{20})}\]\[\sum_{b\geq{0}}(p^{26}t^{14})^{b}=\frac{(1)}{(1-p^{26}t^{14})}\]\[\sum_{c\geq{1}}(p^{18}t^{10})^{c}=\frac{(p^{18}t^{10})}{(1-p^{18}t^{10})}\]\[\sum_{d\geq{0}}(p^{11}t^{6})^{d}=\frac{(1)}{(1-p^{11}t^{6})}\]\[\sum_{a\geq{0}}a(p^{37}t^{20})^{a}=\frac{(p^{37}t^{20})}{(1-p^{37}t^{20})^{2}}\]\[\sum_{b\geq{0}}(p^{26}t^{14})^{b}=\frac{(1)}{(1-p^{26}t^{14})}\]\[\sum_{c\geq{1}}(p^{18}t^{10})^{c}=\frac{(p^{18}t^{10})}{(1-p^{18}t^{10})}\]\[\sum_{d\geq{0}}(p^{11}t^{6})^{d}=\frac{(1)}{(1-p^{11}t^{6})}\]\[\sum_{a\geq{0}}(p^{37}t^{20})^{a}=\frac{(1)}{(1-p^{37}t^{20})}\]\[\sum_{b\geq{0}}b(p^{26}t^{14})^{b}=\frac{(p^{26}t^{14})}{(1-p^{26}t^{14})^{2}}\]\[\sum_{c\geq{1}}(p^{18}t^{10})^{c}=\frac{(p^{18}t^{10})}{(1-p^{18}t^{10})}\]\[\sum_{d\geq{0}}(p^{11}t^{6})^{d}=\frac{(1)}{(1-p^{11}t^{6})}\]\[\sum_{a\geq{0}}(p^{37}t^{20})^{a}=\frac{(1)}{(1-p^{37}t^{20})}\]\[\sum_{b\geq{0}}(p^{26}t^{14})^{b}=\frac{(1)}{(1-p^{26}t^{14})}\]\[\sum_{c\geq{1}}c(p^{18}t^{10})^{c}=\frac{(p^{18}t^{10})}{(1-p^{18}t^{10})^{2}}\]\[\sum_{d\geq{0}}(p^{11}t^{6})^{d}=\frac{(1)}{(1-p^{11}t^{6})}\]\[\sum_{a\geq{0}}a(p^{37}t^{20})^{a}=\frac{(p^{37}t^{20})}{(1-p^{37}t^{20})^{2}}\]\[\sum_{b\geq{0}}b(p^{26}t^{14})^{b}=\frac{(p^{26}t^{14})}{(1-p^{26}t^{14})^{2}}\]\[\sum_{c\geq{1}}(p^{18}t^{10})^{c}=\frac{(p^{18}t^{10})}{(1-p^{18}t^{10})}\]\[\sum_{d\geq{0}}(p^{11}t^{6})^{d}=\frac{(1)}{(1-p^{11}t^{6})}\]\[\sum_{a\geq{0}}a(p^{37}t^{20})^{a}=\frac{(p^{37}t^{20})}{(1-p^{37}t^{20})^{2}}\]\[\sum_{b\geq{0}}(p^{26}t^{14})^{b}=\frac{(1)}{(1-p^{26}t^{14})}\]\[\sum_{c\geq{1}}c(p^{18}t^{10})^{c}=\frac{(p^{18}t^{10})}{(1-p^{18}t^{10})^{2}}\]\[\sum_{d\geq{0}}(p^{11}t^{6})^{d}=\frac{(1)}{(1-p^{11}t^{6})}\]\[\sum_{a\geq{0}}a(p^{37}t^{20})^{a}=\frac{(p^{37}t^{20})}{(1-p^{37}t^{20})^{2}}\]\[\sum_{b\geq{0}}(p^{26}t^{14})^{b}=\frac{(1)}{(1-p^{26}t^{14})}\]\[\sum_{c\geq{1}}(p^{18}t^{10})^{c}=\frac{(p^{18}t^{10})}{(1-p^{18}t^{10})}\]\[\sum_{d\geq{0}}(p^{11}t^{6})^{d}=\frac{(1)}{(1-p^{11}t^{6})}\]\[\frac{(p^{18}t^{10})}{(1-p^{37}t^{20})(1-p^{26}t^{14})(1-p^{18}t^{10})(1-p^{11}t^{6})}\]\[\frac{2(A)(p^{37}t^{20})(p^{18}t^{10})}{(1-p^{37}t^{20})^{2}(1-p^{26}t^{14})(1-p^{18}t^{10})(1-p^{11}t^{6})}\]\[\frac{(A)(p^{26}t^{14})(p^{18}t^{10})}{(1-p^{37}t^{20})(1-p^{26}t^{14})^{2}(1-p^{18}t^{10})(1-p^{11}t^{6})}\]\[\frac{(A)(p^{18}t^{10})}{(1-p^{37}t^{20})(1-p^{26}t^{14})(1-p^{18}t^{10})^{2}(1-p^{11}t^{6})}\]\[\frac{(A^{2})(p^{37}t^{20})(p^{26}t^{14})(p^{18}t^{10})}{(1-p^{37}t^{20})^{2}(1-p^{26}t^{14})^{2}(1-p^{18}t^{10})(1-p^{11}t^{6})}\]\[\frac{(A^{2})(p^{37}t^{20})(p^{18}t^{10})}{(1-p^{37}t^{20})^{2}(1-p^{26}t^{14})(1-p^{18}t^{10})^{2}(1-p^{11}t^{6})}\]\[\frac{(A^{2})(p^{37}t^{20})(p^{18}t^{10})}{(1-p^{37}t^{20})^{2}(1-p^{26}t^{14})(1-p^{18}t^{10})(1-p^{11}t^{6})}\]\[+\frac{(p^{18}t^{10})(1-p^{37}t^{20})(1-p^{26}t^{14})(1-p^{18}t^{10})}{(1-p^{37}t^{20})^{2}(1-p^{26}t^{14})^{2}(1-p^{18}t^{10})^{2}(1-p^{11}t^{6})}+\]\[+\frac{2(A)(p^{37}t^{20})(p^{18}t^{10})(1-p^{26}t^{14})(1-p^{18}t^{10})}{(1-p^{37}t^{20})^{2}(1-p^{26}t^{14})^{2}(1-p^{18}t^{10})^{2}(1-p^{11}t^{6})}+\]\[+\frac{(A)(p^{26}t^{14})(p^{18}t^{10})(1-p^{37}t^{20})(1-p^{18}t^{10})}{(1-p^{37}t^{20})^{2}(1-p^{26}t^{14})^{2}(1-p^{18}t^{10})^{2}(1-p^{11}t^{6})}+\]\[+\frac{(A)(p^{18}t^{10})(1-p^{37}t^{20})(1-p^{26}t^{14})}{(1-p^{37}t^{20})^{2}(1-p^{26}t^{14})^{2}(1-p^{18}t^{10})^{2}(1-p^{11}t^{6})}+\]\[+\frac{(A)^{2}(p^{37}t^{20})(p^{26}t^{14})(p^{18}t^{10})(1-p^{18}t^{10})}{(1-p^{37}t^{20})^{2}(1-p^{26}t^{14})^{2}(1-p^{18}t^{10})^{2}(1-p^{11}t^{6})}+\]\[+\frac{(A)^{2}(p^{37}t^{20})(p^{18}t^{10})(1-p^{26}t^{14})}{(1-p^{37}t^{20})^{2}(1-p^{26}t^{14})^{2}(1-p^{18}t^{10})^{2}(1-p^{11}t^{6})}+\]\[+\frac{(A)^{2}(p^{37}t^{20})(p^{18}t^{10})(1-p^{26}t^{14})(1-p^{18}t^{10})}{(1-p^{37}t^{20})^{2}(1-p^{26}t^{14})^{2}(1-p^{18}t^{10})^{2}(1-p^{11}t^{6})}+\]\end{document}