
                \documentclass{article}
                \usepackage{graphicx} % Required for inserting images
                \usepackage{xcolor}
                \begin{document}
                \[1+(A)v_2+(A)v_3+(A)^2v_2v_3\]\[v_1\rightarrow{2a+b+c+d}\]\[v_2\rightarrow{a}\]\[v_3\rightarrow{a+b+c}\]\[v_4\rightarrow{a+b}\]\[1+2(A)a+(A)b+(A)c+(A)^2a^{2}+(A)^2ab+(A)^2ac\]All series and their sums\[\sum_{a\geq{0}}(p^{44}t^{24})^{a}\sum_{b\geq{1}}(p^{26}t^{14})^{b}\sum_{c\geq{0}}(p^{18}t^{10})^{c}\sum_{d\geq{0}}(p^{7}t^{4})^{d}=\frac{(p^{26}t^{14})}{(1-p^{44}t^{24})(1-p^{26}t^{14})(1-p^{18}t^{10})(1-p^{7}t^{4})}\]\[2(A)\sum_{a\geq{0}}\textcolor{red}{a}(p^{44}t^{24})^{a}\sum_{b\geq{1}}(p^{26}t^{14})^{b}\sum_{c\geq{0}}(p^{18}t^{10})^{c}\sum_{d\geq{0}}(p^{7}t^{4})^{d}=\frac{2(A)(p^{44}t^{24})(p^{26}t^{14})}{(1-p^{44}t^{24})^{\textcolor{red}{2}}(1-p^{26}t^{14})(1-p^{18}t^{10})(1-p^{7}t^{4})}\]\[(A)\sum_{a\geq{0}}(p^{44}t^{24})^{a}\sum_{b\geq{1}}\textcolor{red}{b}(p^{26}t^{14})^{b}\sum_{c\geq{0}}(p^{18}t^{10})^{c}\sum_{d\geq{0}}(p^{7}t^{4})^{d}=\frac{(A)(p^{26}t^{14})}{(1-p^{44}t^{24})(1-p^{26}t^{14})^{\textcolor{red}{2}}(1-p^{18}t^{10})(1-p^{7}t^{4})}\]\[(A)\sum_{a\geq{0}}(p^{44}t^{24})^{a}\sum_{b\geq{1}}(p^{26}t^{14})^{b}\sum_{c\geq{0}}\textcolor{red}{c}(p^{18}t^{10})^{c}\sum_{d\geq{0}}(p^{7}t^{4})^{d}=\frac{(A)(p^{26}t^{14})(p^{18}t^{10})}{(1-p^{44}t^{24})(1-p^{26}t^{14})(1-p^{18}t^{10})^{\textcolor{red}{2}}(1-p^{7}t^{4})}\]\[(A)^{2}\sum_{a\geq{0}}\textcolor{red}{a^{2}}(p^{44}t^{24})^{a}\sum_{b\geq{1}}(p^{26}t^{14})^{b}\sum_{c\geq{0}}(p^{18}t^{10})^{c}\sum_{d\geq{0}}(p^{7}t^{4})^{d}=\frac{(A^{2})(p^{88}t^{48}+p^{44}t^{24})(p^{26}t^{14})}{(1-p^{44}t^{24})^{\textcolor{red}{3}}(1-p^{26}t^{14})(1-p^{18}t^{10})(1-p^{7}t^{4})}\]\[(A)^{2}\sum_{a\geq{0}}\textcolor{red}{a}(p^{44}t^{24})^{a}\sum_{b\geq{1}}\textcolor{red}{b}(p^{26}t^{14})^{b}\sum_{c\geq{0}}(p^{18}t^{10})^{c}\sum_{d\geq{0}}(p^{7}t^{4})^{d}=\frac{(A^{2})(p^{44}t^{24})(p^{26}t^{14})}{(1-p^{44}t^{24})^{\textcolor{red}{2}}(1-p^{26}t^{14})^{\textcolor{red}{2}}(1-p^{18}t^{10})(1-p^{7}t^{4})}\]\[(A)^{2}\sum_{a\geq{0}}\textcolor{red}{a}(p^{44}t^{24})^{a}\sum_{b\geq{1}}(p^{26}t^{14})^{b}\sum_{c\geq{0}}\textcolor{red}{c}(p^{18}t^{10})^{c}\sum_{d\geq{0}}(p^{7}t^{4})^{d}=\frac{(A^{2})(p^{44}t^{24})(p^{26}t^{14})(p^{18}t^{10})}{(1-p^{44}t^{24})^{\textcolor{red}{2}}(1-p^{26}t^{14})(1-p^{18}t^{10})^{\textcolor{red}{2}}(1-p^{7}t^{4})}\]\[+\frac{(p^{26}t^{14})(1-p^{44}t^{24})^{\textcolor{red}{2}}(1-p^{26}t^{14})(1-p^{18}t^{10})}{(1-p^{44}t^{24})^{\textcolor{red}{3}}(1-p^{26}t^{14})^{\textcolor{red}{2}}(1-p^{18}t^{10})^{\textcolor{red}{2}}(1-p^{7}t^{4})}\]\[+\frac{2(A)(p^{44}t^{24})(p^{26}t^{14})(1-p^{26}t^{14})(1-p^{18}t^{10})(1-p^{44}t^{24})}{(1-p^{44}t^{24})^{\textcolor{red}{3}}(1-p^{26}t^{14})^{\textcolor{red}{2}}(1-p^{18}t^{10})^{\textcolor{red}{2}}(1-p^{7}t^{4})}\]\[+\frac{(A)(p^{26}t^{14})(1-p^{44}t^{24})^{\textcolor{red}{2}}(1-p^{18}t^{10})}{(1-p^{44}t^{24})^{\textcolor{red}{3}}(1-p^{26}t^{14})^{\textcolor{red}{2}}(1-p^{18}t^{10})^{\textcolor{red}{2}}(1-p^{7}t^{4})}\]\[+\frac{(A)(p^{26}t^{14})(p^{18}t^{10})(1-p^{44}t^{24})^{\textcolor{red}{2}}(1-p^{26}t^{14})}{(1-p^{44}t^{24})^{\textcolor{red}{3}}(1-p^{26}t^{14})^{\textcolor{red}{2}}(1-p^{18}t^{10})^{\textcolor{red}{2}}(1-p^{7}t^{4})}\]\[+\frac{(A)^{2}(p^{88}t^{48}+p^{44}t^{24})(p^{26}t^{14})(1-p^{26}t^{14})(1-p^{18}t^{10})}{(1-p^{44}t^{24})^{\textcolor{red}{3}}(1-p^{26}t^{14})^{\textcolor{red}{2}}(1-p^{18}t^{10})^{\textcolor{red}{2}}(1-p^{7}t^{4})}\]\[+\frac{(A)^{2}(p^{44}t^{24})(p^{26}t^{14})(1-p^{44}t^{24})(1-p^{18}t^{10})}{(1-p^{44}t^{24})^{\textcolor{red}{3}}(1-p^{26}t^{14})^{\textcolor{red}{2}}(1-p^{18}t^{10})^{\textcolor{red}{2}}(1-p^{7}t^{4})}\]\[+\frac{(A)^{2}(p^{44}t^{24})(p^{26}t^{14})(p^{18}t^{10})(1-p^{44}t^{24})(1-p^{26}t^{14})}{(1-p^{44}t^{24})^{\textcolor{red}{3}}(1-p^{26}t^{14})^{\textcolor{red}{2}}(1-p^{18}t^{10})^{\textcolor{red}{2}}(1-p^{7}t^{4})}\]\[1+(A)v_2+(A)v_3+(A)^2v_2v_3\]\[v_1\rightarrow{a+2b+2c+d}\]\[v_2\rightarrow{b+c}\]\[v_3\rightarrow{a+b+c}\]\[v_4\rightarrow{a+2b+c}\]\[1+2(A)b+2(A)c+(A)a+(A)^2ba+(A)^2ca+(A)^2b^{2}+2(A)^2cb+(A)^2c^{2}\]All series and their sums\[\sum_{a\geq{1}}(p^{26}t^{14})^{a}\sum_{b\geq{1}}(p^{52}t^{28})^{b}\sum_{c\geq{0}}(p^{44}t^{24})^{c}\sum_{d\geq{0}}(p^{7}t^{4})^{d}=\frac{(p^{26}t^{14})(p^{52}t^{28})}{(1-p^{26}t^{14})(1-p^{52}t^{28})(1-p^{44}t^{24})(1-p^{7}t^{4})}\]\[2(A)\sum_{a\geq{1}}(p^{26}t^{14})^{a}\sum_{b\geq{1}}\textcolor{red}{b}(p^{52}t^{28})^{b}\sum_{c\geq{0}}(p^{44}t^{24})^{c}\sum_{d\geq{0}}(p^{7}t^{4})^{d}=\frac{2(A)(p^{26}t^{14})(p^{52}t^{28})}{(1-p^{26}t^{14})(1-p^{52}t^{28})^{\textcolor{red}{2}}(1-p^{44}t^{24})(1-p^{7}t^{4})}\]\[2(A)\sum_{a\geq{1}}(p^{26}t^{14})^{a}\sum_{b\geq{1}}(p^{52}t^{28})^{b}\sum_{c\geq{0}}\textcolor{red}{c}(p^{44}t^{24})^{c}\sum_{d\geq{0}}(p^{7}t^{4})^{d}=\frac{2(A)(p^{26}t^{14})(p^{52}t^{28})(p^{44}t^{24})}{(1-p^{26}t^{14})(1-p^{52}t^{28})(1-p^{44}t^{24})^{\textcolor{red}{2}}(1-p^{7}t^{4})}\]\[(A)\sum_{a\geq{1}}\textcolor{red}{a}(p^{26}t^{14})^{a}\sum_{b\geq{1}}(p^{52}t^{28})^{b}\sum_{c\geq{0}}(p^{44}t^{24})^{c}\sum_{d\geq{0}}(p^{7}t^{4})^{d}=\frac{(A)(p^{26}t^{14})(p^{52}t^{28})}{(1-p^{26}t^{14})^{\textcolor{red}{2}}(1-p^{52}t^{28})(1-p^{44}t^{24})(1-p^{7}t^{4})}\]\[(A)^{2}\sum_{a\geq{1}}\textcolor{red}{a}(p^{26}t^{14})^{a}\sum_{b\geq{1}}\textcolor{red}{b}(p^{52}t^{28})^{b}\sum_{c\geq{0}}(p^{44}t^{24})^{c}\sum_{d\geq{0}}(p^{7}t^{4})^{d}=\frac{(A^{2})(p^{26}t^{14})(p^{52}t^{28})}{(1-p^{26}t^{14})^{\textcolor{red}{2}}(1-p^{52}t^{28})^{\textcolor{red}{2}}(1-p^{44}t^{24})(1-p^{7}t^{4})}\]\[(A)^{2}\sum_{a\geq{1}}\textcolor{red}{a}(p^{26}t^{14})^{a}\sum_{b\geq{1}}(p^{52}t^{28})^{b}\sum_{c\geq{0}}\textcolor{red}{c}(p^{44}t^{24})^{c}\sum_{d\geq{0}}(p^{7}t^{4})^{d}=\frac{(A^{2})(p^{26}t^{14})(p^{52}t^{28})(p^{44}t^{24})}{(1-p^{26}t^{14})^{\textcolor{red}{2}}(1-p^{52}t^{28})(1-p^{44}t^{24})^{\textcolor{red}{2}}(1-p^{7}t^{4})}\]\[(A)^{2}\sum_{a\geq{1}}(p^{26}t^{14})^{a}\sum_{b\geq{1}}\textcolor{red}{b^{2}}(p^{52}t^{28})^{b}\sum_{c\geq{0}}(p^{44}t^{24})^{c}\sum_{d\geq{0}}(p^{7}t^{4})^{d}=\frac{(A^{2})(p^{26}t^{14})(p^{104}t^{56}+p^{52}t^{28})}{(1-p^{26}t^{14})(1-p^{52}t^{28})^{\textcolor{red}{3}}(1-p^{44}t^{24})(1-p^{7}t^{4})}\]\[2(A)^{2}\sum_{a\geq{1}}(p^{26}t^{14})^{a}\sum_{b\geq{1}}\textcolor{red}{b}(p^{52}t^{28})^{b}\sum_{c\geq{0}}\textcolor{red}{c}(p^{44}t^{24})^{c}\sum_{d\geq{0}}(p^{7}t^{4})^{d}=\frac{2(A^{2})(p^{26}t^{14})(p^{52}t^{28})(p^{44}t^{24})}{(1-p^{26}t^{14})(1-p^{52}t^{28})^{\textcolor{red}{2}}(1-p^{44}t^{24})^{\textcolor{red}{2}}(1-p^{7}t^{4})}\]\[(A)^{2}\sum_{a\geq{1}}(p^{26}t^{14})^{a}\sum_{b\geq{1}}(p^{52}t^{28})^{b}\sum_{c\geq{0}}\textcolor{red}{c^{2}}(p^{44}t^{24})^{c}\sum_{d\geq{0}}(p^{7}t^{4})^{d}=\frac{(A^{2})(p^{26}t^{14})(p^{52}t^{28})(p^{88}t^{48}+p^{44}t^{24})}{(1-p^{26}t^{14})(1-p^{52}t^{28})(1-p^{44}t^{24})^{\textcolor{red}{3}}(1-p^{7}t^{4})}\]\[+\frac{(p^{26}t^{14})(p^{52}t^{28})(1-p^{52}t^{28})^{\textcolor{red}{2}}(1-p^{44}t^{24})^{\textcolor{red}{2}}(1-p^{26}t^{14})}{(1-p^{26}t^{14})^{\textcolor{red}{2}}(1-p^{52}t^{28})^{\textcolor{red}{3}}(1-p^{44}t^{24})^{\textcolor{red}{3}}(1-p^{7}t^{4})}\]\[+\frac{2(A)(p^{26}t^{14})(p^{52}t^{28})(1-p^{44}t^{24})^{\textcolor{red}{2}}(1-p^{26}t^{14})(1-p^{52}t^{28})}{(1-p^{26}t^{14})^{\textcolor{red}{2}}(1-p^{52}t^{28})^{\textcolor{red}{3}}(1-p^{44}t^{24})^{\textcolor{red}{3}}(1-p^{7}t^{4})}\]\[+\frac{2(A)(p^{26}t^{14})(p^{52}t^{28})(p^{44}t^{24})(1-p^{52}t^{28})^{\textcolor{red}{2}}(1-p^{26}t^{14})(1-p^{44}t^{24})}{(1-p^{26}t^{14})^{\textcolor{red}{2}}(1-p^{52}t^{28})^{\textcolor{red}{3}}(1-p^{44}t^{24})^{\textcolor{red}{3}}(1-p^{7}t^{4})}\]\[+\frac{(A)(p^{26}t^{14})(p^{52}t^{28})(1-p^{52}t^{28})^{\textcolor{red}{2}}(1-p^{44}t^{24})^{\textcolor{red}{2}}}{(1-p^{26}t^{14})^{\textcolor{red}{2}}(1-p^{52}t^{28})^{\textcolor{red}{3}}(1-p^{44}t^{24})^{\textcolor{red}{3}}(1-p^{7}t^{4})}\]\[+\frac{(A)^{2}(p^{26}t^{14})(p^{52}t^{28})(1-p^{44}t^{24})^{\textcolor{red}{2}}(1-p^{52}t^{28})}{(1-p^{26}t^{14})^{\textcolor{red}{2}}(1-p^{52}t^{28})^{\textcolor{red}{3}}(1-p^{44}t^{24})^{\textcolor{red}{3}}(1-p^{7}t^{4})}\]\[+\frac{(A)^{2}(p^{26}t^{14})(p^{52}t^{28})(p^{44}t^{24})(1-p^{52}t^{28})^{\textcolor{red}{2}}(1-p^{44}t^{24})}{(1-p^{26}t^{14})^{\textcolor{red}{2}}(1-p^{52}t^{28})^{\textcolor{red}{3}}(1-p^{44}t^{24})^{\textcolor{red}{3}}(1-p^{7}t^{4})}\]\[+\frac{(A)^{2}(p^{26}t^{14})(p^{104}t^{56}+p^{52}t^{28})(1-p^{26}t^{14})(1-p^{44}t^{24})^{\textcolor{red}{2}}}{(1-p^{26}t^{14})^{\textcolor{red}{2}}(1-p^{52}t^{28})^{\textcolor{red}{3}}(1-p^{44}t^{24})^{\textcolor{red}{3}}(1-p^{7}t^{4})}\]\[+\frac{2(A)^{2}(p^{26}t^{14})(p^{52}t^{28})(p^{44}t^{24})(1-p^{26}t^{14})(1-p^{52}t^{28})(1-p^{44}t^{24})}{(1-p^{26}t^{14})^{\textcolor{red}{2}}(1-p^{52}t^{28})^{\textcolor{red}{3}}(1-p^{44}t^{24})^{\textcolor{red}{3}}(1-p^{7}t^{4})}\]\[+\frac{(A)^{2}(p^{26}t^{14})(p^{52}t^{28})(p^{88}t^{48}+p^{44}t^{24})(1-p^{26}t^{14})(1-p^{52}t^{28})^{\textcolor{red}{2}}}{(1-p^{26}t^{14})^{\textcolor{red}{2}}(1-p^{52}t^{28})^{\textcolor{red}{3}}(1-p^{44}t^{24})^{\textcolor{red}{3}}(1-p^{7}t^{4})}\]\[1+(A)v_2+(A)v_3+(A)^2v_2v_3\]\[v_1\rightarrow{a+2b+2c+d}\]\[v_2\rightarrow{a+b+c}\]\[v_3\rightarrow{b+c}\]\[v_4\rightarrow{a+2b+c}\]\[1+(A)a+2(A)b+2(A)c+(A)^2ab+(A)^2b^{2}+2(A)^2cb+(A)^2ac+(A)^2c^{2}\]All series and their sums\[\sum_{a\geq{0}}(p^{26}t^{14})^{a}\sum_{b\geq{1}}(p^{52}t^{28})^{b}\sum_{c\geq{0}}(p^{44}t^{24})^{c}\sum_{d\geq{1}}(p^{7}t^{4})^{d}=\frac{(p^{52}t^{28})(p^{7}t^{4})}{(1-p^{26}t^{14})(1-p^{52}t^{28})(1-p^{44}t^{24})(1-p^{7}t^{4})}\]\[(A)\sum_{a\geq{0}}\textcolor{red}{a}(p^{26}t^{14})^{a}\sum_{b\geq{1}}(p^{52}t^{28})^{b}\sum_{c\geq{0}}(p^{44}t^{24})^{c}\sum_{d\geq{1}}(p^{7}t^{4})^{d}=\frac{(A)(p^{26}t^{14})(p^{52}t^{28})(p^{7}t^{4})}{(1-p^{26}t^{14})^{\textcolor{red}{2}}(1-p^{52}t^{28})(1-p^{44}t^{24})(1-p^{7}t^{4})}\]\[2(A)\sum_{a\geq{0}}(p^{26}t^{14})^{a}\sum_{b\geq{1}}\textcolor{red}{b}(p^{52}t^{28})^{b}\sum_{c\geq{0}}(p^{44}t^{24})^{c}\sum_{d\geq{1}}(p^{7}t^{4})^{d}=\frac{2(A)(p^{52}t^{28})(p^{7}t^{4})}{(1-p^{26}t^{14})(1-p^{52}t^{28})^{\textcolor{red}{2}}(1-p^{44}t^{24})(1-p^{7}t^{4})}\]\[2(A)\sum_{a\geq{0}}(p^{26}t^{14})^{a}\sum_{b\geq{1}}(p^{52}t^{28})^{b}\sum_{c\geq{0}}\textcolor{red}{c}(p^{44}t^{24})^{c}\sum_{d\geq{1}}(p^{7}t^{4})^{d}=\frac{2(A)(p^{52}t^{28})(p^{44}t^{24})(p^{7}t^{4})}{(1-p^{26}t^{14})(1-p^{52}t^{28})(1-p^{44}t^{24})^{\textcolor{red}{2}}(1-p^{7}t^{4})}\]\[(A)^{2}\sum_{a\geq{0}}\textcolor{red}{a}(p^{26}t^{14})^{a}\sum_{b\geq{1}}\textcolor{red}{b}(p^{52}t^{28})^{b}\sum_{c\geq{0}}(p^{44}t^{24})^{c}\sum_{d\geq{1}}(p^{7}t^{4})^{d}=\frac{(A^{2})(p^{26}t^{14})(p^{52}t^{28})(p^{7}t^{4})}{(1-p^{26}t^{14})^{\textcolor{red}{2}}(1-p^{52}t^{28})^{\textcolor{red}{2}}(1-p^{44}t^{24})(1-p^{7}t^{4})}\]\[(A)^{2}\sum_{a\geq{0}}(p^{26}t^{14})^{a}\sum_{b\geq{1}}\textcolor{red}{b^{2}}(p^{52}t^{28})^{b}\sum_{c\geq{0}}(p^{44}t^{24})^{c}\sum_{d\geq{1}}(p^{7}t^{4})^{d}=\frac{(A^{2})(p^{104}t^{56}+p^{52}t^{28})(p^{7}t^{4})}{(1-p^{26}t^{14})(1-p^{52}t^{28})^{\textcolor{red}{3}}(1-p^{44}t^{24})(1-p^{7}t^{4})}\]\[2(A)^{2}\sum_{a\geq{0}}(p^{26}t^{14})^{a}\sum_{b\geq{1}}\textcolor{red}{b}(p^{52}t^{28})^{b}\sum_{c\geq{0}}\textcolor{red}{c}(p^{44}t^{24})^{c}\sum_{d\geq{1}}(p^{7}t^{4})^{d}=\frac{2(A^{2})(p^{52}t^{28})(p^{44}t^{24})(p^{7}t^{4})}{(1-p^{26}t^{14})(1-p^{52}t^{28})^{\textcolor{red}{2}}(1-p^{44}t^{24})^{\textcolor{red}{2}}(1-p^{7}t^{4})}\]\[(A)^{2}\sum_{a\geq{0}}\textcolor{red}{a}(p^{26}t^{14})^{a}\sum_{b\geq{1}}(p^{52}t^{28})^{b}\sum_{c\geq{0}}\textcolor{red}{c}(p^{44}t^{24})^{c}\sum_{d\geq{1}}(p^{7}t^{4})^{d}=\frac{(A^{2})(p^{26}t^{14})(p^{52}t^{28})(p^{44}t^{24})(p^{7}t^{4})}{(1-p^{26}t^{14})^{\textcolor{red}{2}}(1-p^{52}t^{28})(1-p^{44}t^{24})^{\textcolor{red}{2}}(1-p^{7}t^{4})}\]\[(A)^{2}\sum_{a\geq{0}}(p^{26}t^{14})^{a}\sum_{b\geq{1}}(p^{52}t^{28})^{b}\sum_{c\geq{0}}\textcolor{red}{c^{2}}(p^{44}t^{24})^{c}\sum_{d\geq{1}}(p^{7}t^{4})^{d}=\frac{(A^{2})(p^{52}t^{28})(p^{88}t^{48}+p^{44}t^{24})(p^{7}t^{4})}{(1-p^{26}t^{14})(1-p^{52}t^{28})(1-p^{44}t^{24})^{\textcolor{red}{3}}(1-p^{7}t^{4})}\]\[+\frac{(p^{52}t^{28})(p^{7}t^{4})(1-p^{26}t^{14})(1-p^{52}t^{28})^{\textcolor{red}{2}}(1-p^{44}t^{24})^{\textcolor{red}{2}}}{(1-p^{26}t^{14})^{\textcolor{red}{2}}(1-p^{52}t^{28})^{\textcolor{red}{3}}(1-p^{44}t^{24})^{\textcolor{red}{3}}(1-p^{7}t^{4})}\]\[+\frac{(A)(p^{26}t^{14})(p^{52}t^{28})(p^{7}t^{4})(1-p^{52}t^{28})^{\textcolor{red}{2}}(1-p^{44}t^{24})^{\textcolor{red}{2}}}{(1-p^{26}t^{14})^{\textcolor{red}{2}}(1-p^{52}t^{28})^{\textcolor{red}{3}}(1-p^{44}t^{24})^{\textcolor{red}{3}}(1-p^{7}t^{4})}\]\[+\frac{2(A)(p^{52}t^{28})(p^{7}t^{4})(1-p^{26}t^{14})(1-p^{44}t^{24})^{\textcolor{red}{2}}(1-p^{52}t^{28})}{(1-p^{26}t^{14})^{\textcolor{red}{2}}(1-p^{52}t^{28})^{\textcolor{red}{3}}(1-p^{44}t^{24})^{\textcolor{red}{3}}(1-p^{7}t^{4})}\]\[+\frac{2(A)(p^{52}t^{28})(p^{44}t^{24})(p^{7}t^{4})(1-p^{26}t^{14})(1-p^{52}t^{28})^{\textcolor{red}{2}}(1-p^{44}t^{24})}{(1-p^{26}t^{14})^{\textcolor{red}{2}}(1-p^{52}t^{28})^{\textcolor{red}{3}}(1-p^{44}t^{24})^{\textcolor{red}{3}}(1-p^{7}t^{4})}\]\[+\frac{(A)^{2}(p^{26}t^{14})(p^{52}t^{28})(p^{7}t^{4})(1-p^{44}t^{24})^{\textcolor{red}{2}}(1-p^{52}t^{28})}{(1-p^{26}t^{14})^{\textcolor{red}{2}}(1-p^{52}t^{28})^{\textcolor{red}{3}}(1-p^{44}t^{24})^{\textcolor{red}{3}}(1-p^{7}t^{4})}\]\[+\frac{(A)^{2}(p^{104}t^{56}+p^{52}t^{28})(p^{7}t^{4})(1-p^{26}t^{14})(1-p^{44}t^{24})^{\textcolor{red}{2}}}{(1-p^{26}t^{14})^{\textcolor{red}{2}}(1-p^{52}t^{28})^{\textcolor{red}{3}}(1-p^{44}t^{24})^{\textcolor{red}{3}}(1-p^{7}t^{4})}\]\[+\frac{2(A)^{2}(p^{52}t^{28})(p^{44}t^{24})(p^{7}t^{4})(1-p^{26}t^{14})(1-p^{52}t^{28})(1-p^{44}t^{24})}{(1-p^{26}t^{14})^{\textcolor{red}{2}}(1-p^{52}t^{28})^{\textcolor{red}{3}}(1-p^{44}t^{24})^{\textcolor{red}{3}}(1-p^{7}t^{4})}\]\[+\frac{(A)^{2}(p^{26}t^{14})(p^{52}t^{28})(p^{44}t^{24})(p^{7}t^{4})(1-p^{52}t^{28})^{\textcolor{red}{2}}(1-p^{44}t^{24})}{(1-p^{26}t^{14})^{\textcolor{red}{2}}(1-p^{52}t^{28})^{\textcolor{red}{3}}(1-p^{44}t^{24})^{\textcolor{red}{3}}(1-p^{7}t^{4})}\]\[+\frac{(A)^{2}(p^{52}t^{28})(p^{88}t^{48}+p^{44}t^{24})(p^{7}t^{4})(1-p^{26}t^{14})(1-p^{52}t^{28})^{\textcolor{red}{2}}}{(1-p^{26}t^{14})^{\textcolor{red}{2}}(1-p^{52}t^{28})^{\textcolor{red}{3}}(1-p^{44}t^{24})^{\textcolor{red}{3}}(1-p^{7}t^{4})}\]\[1+(A)v_2+(A)v_3+(A)^2v_2v_3\]\[v_1\rightarrow{2a+b+c+d}\]\[v_2\rightarrow{a+b}\]\[v_3\rightarrow{a}\]\[v_4\rightarrow{2a+b+c}\]\[1+2(A)a+(A)b+(A)^2a^{2}+(A)^2ba\]All series and their sums\[\sum_{a\geq{0}}(p^{52}t^{28})^{a}\sum_{b\geq{0}}(p^{26}t^{14})^{b}\sum_{c\geq{1}}(p^{15}t^{8})^{c}\sum_{d\geq{0}}(p^{7}t^{4})^{d}=\frac{(p^{15}t^{8})}{(1-p^{52}t^{28})(1-p^{26}t^{14})(1-p^{15}t^{8})(1-p^{7}t^{4})}\]\[2(A)\sum_{a\geq{0}}\textcolor{red}{a}(p^{52}t^{28})^{a}\sum_{b\geq{0}}(p^{26}t^{14})^{b}\sum_{c\geq{1}}(p^{15}t^{8})^{c}\sum_{d\geq{0}}(p^{7}t^{4})^{d}=\frac{2(A)(p^{52}t^{28})(p^{15}t^{8})}{(1-p^{52}t^{28})^{\textcolor{red}{2}}(1-p^{26}t^{14})(1-p^{15}t^{8})(1-p^{7}t^{4})}\]\[(A)\sum_{a\geq{0}}(p^{52}t^{28})^{a}\sum_{b\geq{0}}\textcolor{red}{b}(p^{26}t^{14})^{b}\sum_{c\geq{1}}(p^{15}t^{8})^{c}\sum_{d\geq{0}}(p^{7}t^{4})^{d}=\frac{(A)(p^{26}t^{14})(p^{15}t^{8})}{(1-p^{52}t^{28})(1-p^{26}t^{14})^{\textcolor{red}{2}}(1-p^{15}t^{8})(1-p^{7}t^{4})}\]\[(A)^{2}\sum_{a\geq{0}}\textcolor{red}{a^{2}}(p^{52}t^{28})^{a}\sum_{b\geq{0}}(p^{26}t^{14})^{b}\sum_{c\geq{1}}(p^{15}t^{8})^{c}\sum_{d\geq{0}}(p^{7}t^{4})^{d}=\frac{(A^{2})(p^{104}t^{56}+p^{52}t^{28})(p^{15}t^{8})}{(1-p^{52}t^{28})^{\textcolor{red}{3}}(1-p^{26}t^{14})(1-p^{15}t^{8})(1-p^{7}t^{4})}\]\[(A)^{2}\sum_{a\geq{0}}\textcolor{red}{a}(p^{52}t^{28})^{a}\sum_{b\geq{0}}\textcolor{red}{b}(p^{26}t^{14})^{b}\sum_{c\geq{1}}(p^{15}t^{8})^{c}\sum_{d\geq{0}}(p^{7}t^{4})^{d}=\frac{(A^{2})(p^{52}t^{28})(p^{26}t^{14})(p^{15}t^{8})}{(1-p^{52}t^{28})^{\textcolor{red}{2}}(1-p^{26}t^{14})^{\textcolor{red}{2}}(1-p^{15}t^{8})(1-p^{7}t^{4})}\]\[+\frac{(p^{15}t^{8})(1-p^{52}t^{28})^{\textcolor{red}{2}}(1-p^{26}t^{14})}{(1-p^{52}t^{28})^{\textcolor{red}{3}}(1-p^{26}t^{14})^{\textcolor{red}{2}}(1-p^{15}t^{8})(1-p^{7}t^{4})}\]\[+\frac{2(A)(p^{52}t^{28})(p^{15}t^{8})(1-p^{26}t^{14})(1-p^{52}t^{28})}{(1-p^{52}t^{28})^{\textcolor{red}{3}}(1-p^{26}t^{14})^{\textcolor{red}{2}}(1-p^{15}t^{8})(1-p^{7}t^{4})}\]\[+\frac{(A)(p^{26}t^{14})(p^{15}t^{8})(1-p^{52}t^{28})^{\textcolor{red}{2}}}{(1-p^{52}t^{28})^{\textcolor{red}{3}}(1-p^{26}t^{14})^{\textcolor{red}{2}}(1-p^{15}t^{8})(1-p^{7}t^{4})}\]\[+\frac{(A)^{2}(p^{104}t^{56}+p^{52}t^{28})(p^{15}t^{8})(1-p^{26}t^{14})}{(1-p^{52}t^{28})^{\textcolor{red}{3}}(1-p^{26}t^{14})^{\textcolor{red}{2}}(1-p^{15}t^{8})(1-p^{7}t^{4})}\]\[+\frac{(A)^{2}(p^{52}t^{28})(p^{26}t^{14})(p^{15}t^{8})(1-p^{52}t^{28})}{(1-p^{52}t^{28})^{\textcolor{red}{3}}(1-p^{26}t^{14})^{\textcolor{red}{2}}(1-p^{15}t^{8})(1-p^{7}t^{4})}\]\[1+(A)v_2+(A)v_3+(A)^2v_2v_3\]\[v_1\rightarrow{2a+b+c+d}\]\[v_2\rightarrow{b}\]\[v_3\rightarrow{a+b}\]\[v_4\rightarrow{2a+b+c}\]\[1+2(A)b+(A)a+(A)^2ba+(A)^2b^{2}\]All series and their sums\[\sum_{a\geq{0}}(p^{41}t^{22})^{a}\sum_{b\geq{1}}(p^{37}t^{20})^{b}\sum_{c\geq{1}}(p^{15}t^{8})^{c}\sum_{d\geq{0}}(p^{7}t^{4})^{d}=\frac{(p^{37}t^{20})(p^{15}t^{8})}{(1-p^{41}t^{22})(1-p^{37}t^{20})(1-p^{15}t^{8})(1-p^{7}t^{4})}\]\[2(A)\sum_{a\geq{0}}(p^{41}t^{22})^{a}\sum_{b\geq{1}}\textcolor{red}{b}(p^{37}t^{20})^{b}\sum_{c\geq{1}}(p^{15}t^{8})^{c}\sum_{d\geq{0}}(p^{7}t^{4})^{d}=\frac{2(A)(p^{37}t^{20})(p^{15}t^{8})}{(1-p^{41}t^{22})(1-p^{37}t^{20})^{\textcolor{red}{2}}(1-p^{15}t^{8})(1-p^{7}t^{4})}\]\[(A)\sum_{a\geq{0}}\textcolor{red}{a}(p^{41}t^{22})^{a}\sum_{b\geq{1}}(p^{37}t^{20})^{b}\sum_{c\geq{1}}(p^{15}t^{8})^{c}\sum_{d\geq{0}}(p^{7}t^{4})^{d}=\frac{(A)(p^{41}t^{22})(p^{37}t^{20})(p^{15}t^{8})}{(1-p^{41}t^{22})^{\textcolor{red}{2}}(1-p^{37}t^{20})(1-p^{15}t^{8})(1-p^{7}t^{4})}\]\[(A)^{2}\sum_{a\geq{0}}\textcolor{red}{a}(p^{41}t^{22})^{a}\sum_{b\geq{1}}\textcolor{red}{b}(p^{37}t^{20})^{b}\sum_{c\geq{1}}(p^{15}t^{8})^{c}\sum_{d\geq{0}}(p^{7}t^{4})^{d}=\frac{(A^{2})(p^{41}t^{22})(p^{37}t^{20})(p^{15}t^{8})}{(1-p^{41}t^{22})^{\textcolor{red}{2}}(1-p^{37}t^{20})^{\textcolor{red}{2}}(1-p^{15}t^{8})(1-p^{7}t^{4})}\]\[(A)^{2}\sum_{a\geq{0}}(p^{41}t^{22})^{a}\sum_{b\geq{1}}\textcolor{red}{b^{2}}(p^{37}t^{20})^{b}\sum_{c\geq{1}}(p^{15}t^{8})^{c}\sum_{d\geq{0}}(p^{7}t^{4})^{d}=\frac{(A^{2})(p^{74}t^{40}+p^{37}t^{20})(p^{15}t^{8})}{(1-p^{41}t^{22})(1-p^{37}t^{20})^{\textcolor{red}{3}}(1-p^{15}t^{8})(1-p^{7}t^{4})}\]\[+\frac{(p^{37}t^{20})(p^{15}t^{8})(1-p^{37}t^{20})^{\textcolor{red}{2}}(1-p^{41}t^{22})}{(1-p^{41}t^{22})^{\textcolor{red}{2}}(1-p^{37}t^{20})^{\textcolor{red}{3}}(1-p^{15}t^{8})(1-p^{7}t^{4})}\]\[+\frac{2(A)(p^{37}t^{20})(p^{15}t^{8})(1-p^{41}t^{22})(1-p^{37}t^{20})}{(1-p^{41}t^{22})^{\textcolor{red}{2}}(1-p^{37}t^{20})^{\textcolor{red}{3}}(1-p^{15}t^{8})(1-p^{7}t^{4})}\]\[+\frac{(A)(p^{41}t^{22})(p^{37}t^{20})(p^{15}t^{8})(1-p^{37}t^{20})^{\textcolor{red}{2}}}{(1-p^{41}t^{22})^{\textcolor{red}{2}}(1-p^{37}t^{20})^{\textcolor{red}{3}}(1-p^{15}t^{8})(1-p^{7}t^{4})}\]\[+\frac{(A)^{2}(p^{41}t^{22})(p^{37}t^{20})(p^{15}t^{8})(1-p^{37}t^{20})}{(1-p^{41}t^{22})^{\textcolor{red}{2}}(1-p^{37}t^{20})^{\textcolor{red}{3}}(1-p^{15}t^{8})(1-p^{7}t^{4})}\]\[+\frac{(A)^{2}(p^{74}t^{40}+p^{37}t^{20})(p^{15}t^{8})(1-p^{41}t^{22})}{(1-p^{41}t^{22})^{\textcolor{red}{2}}(1-p^{37}t^{20})^{\textcolor{red}{3}}(1-p^{15}t^{8})(1-p^{7}t^{4})}\]\end{document}