
                \documentclass{article}
                \usepackage{graphicx} % Required for inserting images
                \usepackage{xcolor}
                \begin{document}
                \[1+(A)v_4+(A)v_1+(A)^2v_4v_1-\frac{1}{2}(A)^2v_1^{2}+\frac{1}{2}(A)^2v_1\]\[v_1\rightarrow{a}\]\[v_2\rightarrow{a+b+c}\]\[v_3\rightarrow{a+d}\]\[v_4\rightarrow{a+b}\]\[1+2(A)a+(A)b+\frac{1}{2}(A)^2a^{2}+(A)^2ba+\frac{1}{2}(A)^2a\]All series and their sums\[\sum_{a\geq{0}}(p^{37}t^{20})^{a}\sum_{b\geq{1}}(p^{18}t^{10})^{b}\sum_{c\geq{0}}(p^{11}t^{6})^{c}\sum_{d\geq{1}}(p^{11}t^{6})^{d}=\frac{(p^{18}t^{10})(p^{11}t^{6})}{(1-p^{37}t^{20})(1-p^{18}t^{10})(1-p^{11}t^{6})^{\textcolor{red}{2}}}\]\[2(A)\sum_{a\geq{0}}\textcolor{red}{a}(p^{37}t^{20})^{a}\sum_{b\geq{1}}(p^{18}t^{10})^{b}\sum_{c\geq{0}}(p^{11}t^{6})^{c}\sum_{d\geq{1}}(p^{11}t^{6})^{d}=\frac{2(A)(p^{37}t^{20})(p^{18}t^{10})(p^{11}t^{6})}{(1-p^{37}t^{20})^{\textcolor{red}{2}}(1-p^{18}t^{10})(1-p^{11}t^{6})^{\textcolor{red}{2}}}\]\[(A)\sum_{a\geq{0}}(p^{37}t^{20})^{a}\sum_{b\geq{1}}\textcolor{red}{b}(p^{18}t^{10})^{b}\sum_{c\geq{0}}(p^{11}t^{6})^{c}\sum_{d\geq{1}}(p^{11}t^{6})^{d}=\frac{(A)(p^{18}t^{10})(p^{11}t^{6})}{(1-p^{37}t^{20})(1-p^{18}t^{10})^{\textcolor{red}{2}}(1-p^{11}t^{6})^{\textcolor{red}{2}}}\]\[\frac{1}{2}(A)^{2}\sum_{a\geq{0}}\textcolor{red}{a^{2}}(p^{37}t^{20})^{a}\sum_{b\geq{1}}(p^{18}t^{10})^{b}\sum_{c\geq{0}}(p^{11}t^{6})^{c}\sum_{d\geq{1}}(p^{11}t^{6})^{d}=\frac{\frac{1}{2}(A^{2})(p^{74}t^{40}+p^{37}t^{20})(p^{18}t^{10})(p^{11}t^{6})}{(1-p^{37}t^{20})^{\textcolor{red}{3}}(1-p^{18}t^{10})(1-p^{11}t^{6})^{\textcolor{red}{2}}}\]\[(A)^{2}\sum_{a\geq{0}}\textcolor{red}{a}(p^{37}t^{20})^{a}\sum_{b\geq{1}}\textcolor{red}{b}(p^{18}t^{10})^{b}\sum_{c\geq{0}}(p^{11}t^{6})^{c}\sum_{d\geq{1}}(p^{11}t^{6})^{d}=\frac{(A^{2})(p^{37}t^{20})(p^{18}t^{10})(p^{11}t^{6})}{(1-p^{37}t^{20})^{\textcolor{red}{2}}(1-p^{18}t^{10})^{\textcolor{red}{2}}(1-p^{11}t^{6})^{\textcolor{red}{2}}}\]\[\frac{1}{2}(A)^{2}\sum_{a\geq{0}}\textcolor{red}{a}(p^{37}t^{20})^{a}\sum_{b\geq{1}}(p^{18}t^{10})^{b}\sum_{c\geq{0}}(p^{11}t^{6})^{c}\sum_{d\geq{1}}(p^{11}t^{6})^{d}=\frac{\frac{1}{2}(A^{2})(p^{37}t^{20})(p^{18}t^{10})(p^{11}t^{6})}{(1-p^{37}t^{20})^{\textcolor{red}{2}}(1-p^{18}t^{10})(1-p^{11}t^{6})^{\textcolor{red}{2}}}\]\[+\frac{(p^{18}t^{10})(p^{11}t^{6})(1-p^{37}t^{20})^{\textcolor{red}{2}}(1-p^{18}t^{10})}{(1-p^{37}t^{20})^{\textcolor{red}{3}}(1-p^{18}t^{10})^{\textcolor{red}{2}}(1-p^{11}t^{6})^{\textcolor{red}{2}}}\]\[+\frac{2(A)(p^{37}t^{20})(p^{18}t^{10})(p^{11}t^{6})(1-p^{18}t^{10})(1-p^{37}t^{20})}{(1-p^{37}t^{20})^{\textcolor{red}{3}}(1-p^{18}t^{10})^{\textcolor{red}{2}}(1-p^{11}t^{6})^{\textcolor{red}{2}}}\]\[+\frac{(A)(p^{18}t^{10})(p^{11}t^{6})(1-p^{37}t^{20})^{\textcolor{red}{2}}}{(1-p^{37}t^{20})^{\textcolor{red}{3}}(1-p^{18}t^{10})^{\textcolor{red}{2}}(1-p^{11}t^{6})^{\textcolor{red}{2}}}\]\[+\frac{\frac{1}{2}(A)^{2}(p^{74}t^{40}+p^{37}t^{20})(p^{18}t^{10})(p^{11}t^{6})(1-p^{18}t^{10})}{(1-p^{37}t^{20})^{\textcolor{red}{3}}(1-p^{18}t^{10})^{\textcolor{red}{2}}(1-p^{11}t^{6})^{\textcolor{red}{2}}}\]\[+\frac{(A)^{2}(p^{37}t^{20})(p^{18}t^{10})(p^{11}t^{6})(1-p^{37}t^{20})}{(1-p^{37}t^{20})^{\textcolor{red}{3}}(1-p^{18}t^{10})^{\textcolor{red}{2}}(1-p^{11}t^{6})^{\textcolor{red}{2}}}\]\[+\frac{\frac{1}{2}(A)^{2}(p^{37}t^{20})(p^{18}t^{10})(p^{11}t^{6})(1-p^{37}t^{20})(1-p^{18}t^{10})}{(1-p^{37}t^{20})^{\textcolor{red}{3}}(1-p^{18}t^{10})^{\textcolor{red}{2}}(1-p^{11}t^{6})^{\textcolor{red}{2}}}\]\end{document}