\documentclass{article}
\usepackage{graphicx} % Required for inserting images
\usepackage{xcolor}
\usepackage{amsmath}
\begin{document}
3.2.1

$p^{v_2}(1+v_1\rho+v_2\rho-\frac{v_1^2}{2}\rho^2+v_4v_1\rho^2-\frac{v_2^2}{2}\rho^2+v_4v_2\rho^2-\frac{v_4^2}{2}\rho^2-\frac{v_1}{2}\rho^2-\frac{v_2}{2}\rho^2+\frac{v_4}{2}\rho^2)$

$f(p,t)=p^{7v_1+10v_2+11v_3+7v_4+v_1}t^{4v_1+6v_2+6v_3+4v_4}=p^{8v_1+10v_2+11v_3+7v_4}t^{4v_1+6v_2+6v_3+4v_4}$

$v_1+v_2\overset{d}{\geq}v_4\overset{c}{>}v_3\overset{b}{>}{v_2}\overset{a}{>}v_1\overset{e}{\geq}{0}$

\[v_1\rightarrow{b+c+d}\]
\[v_2\rightarrow{a+b+c+d}\]
\[v_3\rightarrow{a+2b+c+d}\]
\[v_4\rightarrow{a+2b+2c+d}\]

\[d\geq{0}\]
\[a,b,c\geq{1}\]

\[f(p,t)=p^{(a+b+c+d)}p^{8(b+c+d)+10(a+b+c+d)+11(a+2b+c+d)+7(a+2b+2c+d)}t^{4(b+c+d)+6(a+b+c+d)+6(a+2b+c+d)+4(a+2b+2c+d)}=\]\[=(p^{29}t^{16})^a(p^{55}t^{30})^b(p^{44}t^{24})^c(p^{37}t^{20})^d\]

3.2.1-15

\[-(1-p^{-1})^2\sum_{a\geq{1}}a^2(p^{29}t^{16})^a\sum_{b\geq{1}}(p^{55}t^{30})^b\sum_{c\geq{1}}(p^{44}t^{24})^c\sum_{d\geq{0}}(p^{37}t^{20})^d=\]\[=-(1-p^{-1})^2\frac{(p^{58}t^{32}+p^{29}t^{16})}{(1-p^{29}t^{16})^3}\frac{(p^{55}t^{30})}{(1-p^{55}t^{30})}\frac{(p^{44}t^{24})}{(1-p^{44}t^{24})}\frac{1}{(1-p^{37}t^{20})}\]

@@@@@@@@@@@@@@@@@@@@@@@






2.1.4
\[\sum_{v_{11}\geq{-v_2-v_3}}=p^{v_2}(1+v_2\rho+v_3\rho+v_2v_3\rho^2).\]

\[\Rightarrow{f(p,t)=p^{7v_1+11v_2+11v_3+7v_4+v_4}t^{4v_1+6v_2+6v_3+4v_4}=p^{7v_1+10v_2+11v_3+8v_4}t^{4v_1+6v_2+6v_3+4v_4}}\]

\[v_1\overset{d}{\geq}{v_4}\overset{c}{>}v_2+v_3\overset{a}{\geq}{v_2}\overset{b}{\geq}v_3\overset{a}{\geq}{0}\]

\[v_1\rightarrow{2a+b+c+d}\]
\[v_2\rightarrow{a+b}\]
\[v_3\rightarrow{a}\]
\[v_4\rightarrow{2a+b+c}\]

\[a,b,d\geq{0}\]
\[c\geq{1}\]

\[\Rightarrow{f(p,t)=p^{7(2a+b+c+d)+11(a+b)+11a+8(2a+b+c)}t^{4(2a+b+c+d)+6(a+b)+6a+4(2a+b+c)}}=\]\[=p^{14a+7b+7c+7d+11a+11b+11a+16a+8b+8c}t^{8a+4b+4c+4d+6a+6b+6a+8a+4b+4c}=\]\[=p^{52a+26b+15c+7d}t^{28a+14b+8c+4d}=(p^{52}t^{28})^a(p^{26}t^{14})^b(p^{15}t^{8})^c(p^{7}t^{4})^d\]

\[1+v_2\rho+v_3\rho+v_2v_3\rho^2\rightarrow{1+a\rho+b\rho+a\rho+(a+b)a\rho^2=1+2a\rho+b\rho+a^2\rho^2+ba\rho^2}\]

\[
\sum_{a\geq{0}}(p^{52}t^{28})^a\sum_{b\geq{0}}(p^{26}t^{14})^b\sum_{c\geq{1}}(p^{15}t^{8})^c\sum_{d\geq{0}}(p^{7}t^{4})^d=\]\[=\frac{1}{(1-p^{52}t^{28})}\frac{1}{(1-p^{26}t^{14})}\frac{(p^{15}t^{8})}{(1-p^{15}t^{8})}\frac{1}{(1-p^{7}t^{4})}
\]
\[
+2\rho\sum_{a\geq{0}}a(p^{52}t^{28})^a\sum_{b\geq{0}}(p^{26}t^{14})^b\sum_{c\geq{1}}(p^{15}t^{8})^c\sum_{d\geq{0}}(p^{7}t^{4})^d=\]\[=2\rho\frac{p^{52}t^{28}}{(1-p^{52}t^{28})^2}\frac{1}{(1-p^{26}t^{14})}\frac{(p^{15}t^{8})}{(1-p^{15}t^{8})}\frac{1}{(1-p^{7}t^{4})}
\]
\[
+\rho\sum_{a\geq{0}}(p^{52}t^{28})^a\sum_{b\geq{0}}b(p^{26}t^{14})^b\sum_{c\geq{1}}(p^{15}t^{8})^c\sum_{d\geq{0}}(p^{7}t^{4})^d=\]\[=\rho\frac{1}{(1-p^{52}t^{28})}\frac{p^{26}t^{14}}{(1-p^{26}t^{14})^2}\frac{(p^{15}t^{8})}{(1-p^{15}t^{8})}\frac{1}{(1-p^{7}t^{4})}
\]
\[
+\rho^2\sum_{a\geq{0}}a^2(p^{52}t^{28})^a\sum_{b\geq{0}}(p^{26}t^{14})^b\sum_{c\geq{1}}(p^{15}t^{8})^c\sum_{d\geq{0}}(p^{7}t^{4})^d=\]\[=\rho^2\frac{(p^{52}t^{28})^2+p^{52}t^{28}}{(1-p^{52}t^{28})^3}\frac{1}{(1-p^{26}t^{14})}\frac{(p^{15}t^{8})}{(1-p^{15}t^{8})}\frac{1}{(1-p^{7}t^{4})}
\]
\[
+\rho^2\sum_{a\geq{0}}a(p^{52}t^{28})^a\sum_{b\geq{0}}b(p^{26}t^{14})^b\sum_{c\geq{1}}(p^{15}t^{8})^c\sum_{d\geq{0}}(p^{7}t^{4})^d=\]\[=\rho^2\frac{p^{52}t^{28}}{(1-p^{52}t^{28})^2}\frac{p^{26}t^{14}}{(1-p^{26}t^{14})^2}\frac{(p^{15}t^{8})}{(1-p^{15}t^{8})}\frac{1}{(1-p^{7}t^{4})}
\]
\textbf{Numerator}
\[
(1-p^{52}t^{28})^2(1-p^{26}t^{14})(p^{15}t^{8})+2\rho(p^{52}t^{28})(1-p^{52}t^{28})(1-p^{26}t^{14})(p^{15}t^{8})+\]\[+\rho(1-p^{52}t^{28})^2(p^{26}t^{14})(p^{15}t^{8})+
\rho^2((p^{52}t^{28})^2+p^{52}t^{28})(1-p^{26}t^{14})(p^{15}t^{8})+\]\[+\rho^2(1-p^{52}t^{28})(p^{52}t^{28})(p^{26}t^{14})(p^{15}t^{8})
\]

\textbf{Denominator}
\[(1-p^{52}t^{28})^3(1-p^{26}t^{14})^2(1-p^{15}t^{8})(1-p^{7}t^{4})
\]
\end{document}